Std/Control/ForInStep/Basic.lean
@@ -1,0 +1,34 @@
+/-
+Copyright (c) 2022 Mario Carneiro. All rights reserved.
+Released under Apache 2.0 license as described in the file LICENSE.
+Authors: Mario Carneiro
+-/
+
+/-! # Additional definitions on `ForInStep` -/
+
+/--
+This is similar to a monadic `bind` operator, except that the two type parameters have to be
+the same, which prevents putting a monad instance on `ForInStepT m α := m (ForInStep α)`.
+-/
+@[inline] protected def ForInStep.bind [Monad m]
+    (a : ForInStep α) (f : α → m (ForInStep α)) : m (ForInStep α) :=
+  match a with
+  | .done a => return .done a
+  | .yield a => f a
+
+@[inherit_doc ForInStep.bind] protected abbrev ForInStep.bindM [Monad m]
+    (a : m (ForInStep α)) (f : α → m (ForInStep α)) : m (ForInStep α) := a >>= (·.bind f)
+
+/--
+Get the value out of a `ForInStep`.
+This is usually done at the end of a `forIn` loop to scope the early exit to the loop body.
+-/
+@[inline] def ForInStep.run : ForInStep α → α
+  | .done a
+  | .yield a => a
+
+/-- Applies function `f` to each element of a list to accumulate a `ForInStep` value. -/
+def ForInStep.bindList [Monad m]
+      (f : α → β → m (ForInStep β)) : List α → ForInStep β → m (ForInStep β)
+  | [], s => pure s
+  | a::l, s => s.bind fun b => f a b >>= (·.bindList f l)
